Cleanup in lists and trees.

HOL/DataStrs/RBT_Base.thy
@@ -13,18 +13,18 @@ begin
 section {* Definition of RBT *}
 
 datatype color = R | B
-datatype ('a, 'b) pre_rbt =
+datatype ('a, 'b) rbt =
     Leaf
-  | Node (lsub: "('a, 'b) pre_rbt") (cl: color) (key: 'a) (val: 'b) (rsub: "('a, 'b) pre_rbt")
+  | Node (lsub: "('a, 'b) rbt") (cl: color) (key: 'a) (val: 'b) (rsub: "('a, 'b) rbt")
 where
   "cl Leaf = B"
 
 setup {* add_resolve_prfstep @{thm color.distinct(1)} *}
-setup {* add_resolve_prfstep @{thm pre_rbt.distinct(2)} *}
-setup {* fold add_rewrite_rule @{thms pre_rbt.sel} *}
-setup {* add_forward_prfstep (equiv_forward_th (@{thm pre_rbt.simps(1)})) *}
-setup {* add_forward_prfstep @{thm pre_rbt.collapse} *}
-setup {* add_var_induct_rule @{thm pre_rbt.induct} *}
+setup {* add_resolve_prfstep @{thm rbt.distinct(2)} *}
+setup {* fold add_rewrite_rule @{thms rbt.sel} *}
+setup {* add_forward_prfstep (equiv_forward_th (@{thm rbt.simps(1)})) *}
+setup {* add_forward_prfstep_cond @{thm rbt.collapse} [with_cond "?tree \<noteq> Node ?l ?c ?k ?v ?r"] *}
+setup {* add_var_induct_rule @{thm rbt.induct} *}
 
 lemma not_R [forward]: "c \<noteq> R \<Longrightarrow> c = B" using color.exhaust by blast
 lemma not_B [forward]: "c \<noteq> B \<Longrightarrow> c = R" using color.exhaust by blast
@@ -32,26 +32,26 @@ lemma red_not_leaf [forward]: "cl t = R \<Longrightarrow> t \<noteq> Leaf" by au
 
 section {* RBT invariants *}
 
-fun black_depth :: "('a, 'b) pre_rbt \<Rightarrow> nat" where
+fun black_depth :: "('a, 'b) rbt \<Rightarrow> nat" where
   "black_depth Leaf = 0"
 | "black_depth (Node l R k v r) = black_depth l"
 | "black_depth (Node l B k v r) = black_depth l + 1"
 setup {* fold add_rewrite_rule @{thms black_depth.simps} *}
 
-fun cl_inv :: "('a, 'b) pre_rbt \<Rightarrow> bool" where
+fun cl_inv :: "('a, 'b) rbt \<Rightarrow> bool" where
   "cl_inv Leaf = True"
 | "cl_inv (Node l R k v r) = (cl_inv l \<and> cl_inv r \<and> cl l = B \<and> cl r = B)"
 | "cl_inv (Node l B k v r) = (cl_inv l \<and> cl_inv r)"
 setup {* fold add_rewrite_rule @{thms cl_inv.simps} *}
 setup {* add_property_const @{term cl_inv} *}
 
-fun bd_inv :: "('a, 'b) pre_rbt \<Rightarrow> bool" where
+fun bd_inv :: "('a, 'b) rbt \<Rightarrow> bool" where
   "bd_inv Leaf = True"
 | "bd_inv (Node l c k v r) = (bd_inv l \<and> bd_inv r \<and> black_depth l = black_depth r)"
 setup {* fold add_rewrite_rule @{thms bd_inv.simps} *}
 setup {* add_property_const @{term bd_inv} *}
 
-definition is_rbt :: "('a, 'b) pre_rbt \<Rightarrow> bool" where [rewrite]:
+definition is_rbt :: "('a, 'b) rbt \<Rightarrow> bool" where [rewrite]:
   "is_rbt t = (cl_inv t \<and> bd_inv t)"
 setup {* add_property_const @{term is_rbt} *}
 
@@ -69,12 +69,12 @@ section {* Balancedness of RBT *}
 (* Remove after having general normalization procedure for nats. *)
 lemma two_distrib [rewrite]: "(2::nat) * (a + 1) = 2 * a + 2" by simp
 
-fun min_depth :: "('a, 'b) pre_rbt \<Rightarrow> nat" where
+fun min_depth :: "('a, 'b) rbt \<Rightarrow> nat" where
   "min_depth Leaf = 0"
 | "min_depth (Node l c k v r) = min (min_depth l) (min_depth r) + 1"
 setup {* fold add_rewrite_rule @{thms min_depth.simps} *}
 
-fun max_depth :: "('a, 'b) pre_rbt \<Rightarrow> nat" where
+fun max_depth :: "('a, 'b) rbt \<Rightarrow> nat" where
   "max_depth Leaf = 0"
 | "max_depth (Node l c k v r) = max (max_depth l) (max_depth r) + 1"
 setup {* fold add_rewrite_rule @{thms max_depth.simps} *}
@@ -93,7 +93,7 @@ theorem rbt_balanced: "is_rbt t \<Longrightarrow> max_depth t \<le> 2 * min_dept
 
 section {* Definition and basic properties of cl_inv' *}
 
-fun cl_inv' :: "('a, 'b) pre_rbt \<Rightarrow> bool" where
+fun cl_inv' :: "('a, 'b) rbt \<Rightarrow> bool" where
   "cl_inv' Leaf = True"
 | "cl_inv' (Node l c k v r) = (cl_inv l \<and> cl_inv r)"
 setup {* fold add_rewrite_rule @{thms cl_inv'.simps} *}
@@ -114,17 +114,17 @@ setup {* add_forward_prfstep_cond @{thm cl_inv'I} [with_term "Node ?l ?c ?k ?v ?
 
 subsection {* Set of keys, sortedness *}
 
-fun rbt_in_traverse :: "('a, 'b) pre_rbt \<Rightarrow> 'a list" where
+fun rbt_in_traverse :: "('a, 'b) rbt \<Rightarrow> 'a list" where
   "rbt_in_traverse Leaf = []"
 | "rbt_in_traverse (Node l c k v r) = (rbt_in_traverse l) @ [k] @ (rbt_in_traverse r)"
 setup {* fold add_rewrite_rule @{thms rbt_in_traverse.simps} *}
 
-fun rbt_set :: "('a, 'b) pre_rbt \<Rightarrow> 'a set" where
+fun rbt_set :: "('a, 'b) rbt \<Rightarrow> 'a set" where
   "rbt_set Leaf = {}"
 | "rbt_set (Node l c k v r) = {k} \<union> rbt_set l \<union> rbt_set r"
 setup {* fold add_rewrite_rule @{thms rbt_set.simps} *}
 
-fun rbt_in_traverse_pairs :: "('a, 'b) pre_rbt \<Rightarrow> ('a \<times> 'b) list" where
+fun rbt_in_traverse_pairs :: "('a, 'b) rbt \<Rightarrow> ('a \<times> 'b) list" where
   "rbt_in_traverse_pairs Leaf = []"
 | "rbt_in_traverse_pairs (Node l c k v r) = (rbt_in_traverse_pairs l) @ [(k, v)] @ (rbt_in_traverse_pairs r)"
 setup {* fold add_rewrite_rule @{thms rbt_in_traverse_pairs.simps} *}
@@ -132,11 +132,11 @@ setup {* fold add_rewrite_rule @{thms rbt_in_traverse_pairs.simps} *}
 lemma rbt_in_traverse_fst [rewrite]: "map fst (rbt_in_traverse_pairs t) = rbt_in_traverse t"
 @proof @induct t @qed
 
-definition rbt_map :: "('a, 'b) pre_rbt \<Rightarrow> ('a, 'b) map" where
+definition rbt_map :: "('a, 'b) rbt \<Rightarrow> ('a, 'b) map" where
   "rbt_map t = map_of_alist (rbt_in_traverse_pairs t)"
 setup {* add_rewrite_rule @{thm rbt_map_def} *}
 
-fun rbt_sorted :: "('a::linorder, 'b) pre_rbt \<Rightarrow> bool" where
+fun rbt_sorted :: "('a::linorder, 'b) rbt \<Rightarrow> bool" where
   "rbt_sorted Leaf = True"
 | "rbt_sorted (Node l c k v r) = ((\<forall>x\<in>rbt_set l. x < k) \<and> (\<forall>x\<in>rbt_set r. k < x) \<and> rbt_sorted l \<and> rbt_sorted r)"
 setup {* fold add_rewrite_rule @{thms rbt_sorted.simps} *}
