HOL/DataStrs/Lists_Ex.thy
@@ -20,14 +20,31 @@ setup {* fold add_rewrite_rule @{thms itrev.simps} *}
 
 lemma itrev_eq_rev: "itrev x [] = rev x"
 @proof
-  @have (@rule) "\<forall>y. itrev x y = rev x @ y" @with
-    @induct x arbitrary y @with
-      @subgoal "x = a # b" @have "a # y = [a] @ y" @endgoal
-    @end
+  @induct x for "\<forall>y. itrev x y = rev x @ y" arbitrary y @with
+    @subgoal "x = a # b" @have "a # y = [a] @ y" @endgoal
   @end
 @qed
 
-section {* strict_sorted *}
+section {* Merge sort *}
+
+fun merge_list :: "('a::ord) list \<Rightarrow> 'a list \<Rightarrow> 'a list" where
+  "merge_list xs [] = xs"
+| "merge_list [] ys = ys"
+| "merge_list (x # xs) (y # ys) = (
+    if x \<le> y then x # (merge_list xs (y # ys))
+    else y # (merge_list (x # xs) ys))"
+setup {* fold add_rewrite_rule @{thms merge_list.simps} *}
+setup {* add_fun_induct_rule (@{term_pat "merge_list (?a0.0::?'a::ord list) ?a1.0"}, @{thm merge_list.induct}) *}
+
+lemma merge_list_correct [rewrite]:
+  "set (merge_list xs ys) = set xs \<union> set ys"
+@proof @fun_induct "merge_list xs ys" @qed
+
+lemma merge_list_sorted [forward]:
+  "sorted xs \<Longrightarrow> sorted ys \<Longrightarrow> sorted (merge_list xs ys)"
+@proof @fun_induct "merge_list xs ys" @qed
+
+section {* Strict sorted *}
 
 fun strict_sorted :: "'a::linorder list \<Rightarrow> bool" where
   "strict_sorted [] = True"
@@ -47,22 +64,8 @@ lemma strict_sorted_appendE2 [forward]:
   "strict_sorted (xs @ ys) \<Longrightarrow> x \<in> set xs \<Longrightarrow> \<forall>y\<in>set ys. x < y"
 @proof @induct xs @qed
 
-lemma strict_sorted_distinct [resolve]: "strict_sorted l \<Longrightarrow> distinct l"
+lemma strict_sorted_distinct [forward]: "strict_sorted l \<Longrightarrow> distinct l"
 @proof @induct l @qed
-
-lemma strict_sorted_delmin [rewrite]:
-  "strict_sorted (x # xs) \<Longrightarrow> set (x # xs) - {x} = set xs"
-@proof @have "distinct (x # xs)" @qed
-
-theorem map_of_alist_binary [rewrite]:
-  "strict_sorted (map fst (xs @ [a] @ ys)) \<Longrightarrow> (map_of_alist (xs @ [a] @ ys))\<langle>x\<rangle> =
-   (if x < fst a then (map_of_alist xs)\<langle>x\<rangle>
-    else if x > fst a then (map_of_alist ys)\<langle>x\<rangle> else Some (snd a))"
-@proof
-  @induct xs @with
-    @subgoal "xs = []" @case "x \<notin> set (map fst ys)" @endgoal
-  @end
-@qed
 
 section {* Ordered insert *}
 
@@ -74,20 +77,49 @@ fun ordered_insert :: "'a::ord \<Rightarrow> 'a list \<Rightarrow> 'a list" wher
     else y # ordered_insert x ys)"
 setup {* fold add_rewrite_rule @{thms ordered_insert.simps} *}
 
-theorem ordered_insert_set [rewrite]:
+lemma ordered_insert_set [rewrite]:
   "set (ordered_insert x ys) = {x} \<union> set ys"
 @proof @induct ys @qed
 
-theorem ordered_insert_sorted [backward]:
+lemma ordered_insert_sorted [forward]:
   "strict_sorted ys \<Longrightarrow> strict_sorted (ordered_insert x ys)"
 @proof @induct ys @qed
 
-theorem ordered_insert_binary [rewrite]:
+lemma ordered_insert_binary [rewrite]:
   "strict_sorted (xs @ [a] @ ys) \<Longrightarrow> ordered_insert x (xs @ [a] @ ys) =
     (if x < a then (ordered_insert x xs) @ [a] @ ys
      else if x > a then xs @ [a] @ ordered_insert x ys
      else xs @ [a] @ ys)"
 @proof @induct xs @qed
+
+section {* Deleting an element *}
+
+fun remove_elt_list :: "'a \<Rightarrow> 'a list \<Rightarrow> 'a list" where
+  "remove_elt_list x [] = []"
+| "remove_elt_list x (y # ys) = (if y = x then remove_elt_list x ys else y # remove_elt_list x ys)"
+setup {* fold add_rewrite_rule @{thms remove_elt_list.simps} *}
+
+lemma remove_elt_list_set [rewrite]:
+  "set (remove_elt_list x ys) = set ys - {x}"
+@proof @induct ys @qed
+
+lemma remove_elt_list_sorted [forward]:
+  "strict_sorted ys \<Longrightarrow> strict_sorted (remove_elt_list x ys)"
+@proof @induct ys @qed
+
+lemma remove_elt_idem [rewrite]:
+  "x \<notin> set ys \<Longrightarrow> remove_elt_list x ys = ys"
+@proof @induct ys @qed
+
+lemma remove_elt_list_binary [rewrite]:
+  "strict_sorted (xs @ [a] @ ys) \<Longrightarrow> remove_elt_list x (xs @ [a] @ ys) =
+    (if x < a then (remove_elt_list x xs) @ [a] @ ys
+     else if x > a then xs @ [a] @ remove_elt_list x ys else xs @ ys)"
+@proof @induct xs @with
+  @subgoal "xs = []"
+    @case "x < a" @with @have "x \<notin> set ys" @end
+  @endgoal @end
+@qed
 
 section {* Ordered insertion into list of pairs *}
 
@@ -99,60 +131,27 @@ fun ordered_insert_pairs :: "'a::ord \<Rightarrow> 'b \<Rightarrow> ('a \<times>
     else y # ordered_insert_pairs x v ys)"
 setup {* fold add_rewrite_rule @{thms ordered_insert_pairs.simps} *}
 
-theorem ordered_insert_pairs_map [rewrite]:
+lemma ordered_insert_pairs_map [rewrite]:
   "map_of_alist (ordered_insert_pairs x v ys) = update_map (map_of_alist ys) x v"
 @proof @induct ys @qed
 
-theorem ordered_insert_pairs_set [rewrite]:
+lemma ordered_insert_pairs_set [rewrite]:
   "set (map fst (ordered_insert_pairs x v ys)) = {x} \<union> set (map fst ys)"
 @proof @induct ys @qed
 
-theorem ordered_insert_pairs_sorted [backward]:
+lemma ordered_insert_pairs_sorted [backward]:
   "strict_sorted (map fst ys) \<Longrightarrow> strict_sorted (map fst (ordered_insert_pairs x v ys))"
 @proof @induct ys @qed
 
-theorem ordered_insert_pairs_binary [rewrite]:
+lemma ordered_insert_pairs_binary [rewrite]:
   "strict_sorted (map fst (xs @ [a] @ ys)) \<Longrightarrow> ordered_insert_pairs x v (xs @ [a] @ ys) =
     (if x < fst a then (ordered_insert_pairs x v xs) @ [a] @ ys
      else if x > fst a then xs @ [a] @ ordered_insert_pairs x v ys
      else xs @ [(x, v)] @ ys)"
-@proof
-  @induct xs @with
-    @subgoal "xs = x' # xs'"
-      @case "x < fst a" @then @have "fst a > fst x'"
-    @endgoal
-  @end   
-@qed
-
-section {* Deleting an element *}
-
-fun remove_elt_list :: "'a \<Rightarrow> 'a list \<Rightarrow> 'a list" where
-  "remove_elt_list x [] = []"
-| "remove_elt_list x (y # ys) = (if y = x then remove_elt_list x ys else y # remove_elt_list x ys)"
-setup {* fold add_rewrite_rule @{thms remove_elt_list.simps} *}
-
-theorem remove_elt_list_set [rewrite]:
-  "set (remove_elt_list x ys) = set ys - {x}"
-@proof @induct ys @qed
-
-theorem remove_elt_list_sorted [backward]:
-  "strict_sorted ys \<Longrightarrow> strict_sorted (remove_elt_list x ys)"
-@proof @induct ys @qed
-
-theorem remove_elt_idem [rewrite]:
-  "x \<notin> set xs \<Longrightarrow> remove_elt_list x xs = xs"
-@proof @induct xs @qed
-
-theorem remove_elt_list_binary [rewrite]:
-  "strict_sorted (xs @ [a] @ ys) \<Longrightarrow> remove_elt_list x (xs @ [a] @ ys) =
-    (if x < a then (remove_elt_list x xs) @ [a] @ ys
-     else if x > a then xs @ [a] @ remove_elt_list x ys else xs @ ys)"
-@proof
-  @induct xs @with
-    @subgoal "xs = []"
-      @case "x < a" @with @have "x \<notin> set ys" @end
-    @endgoal
-  @end
+@proof @induct xs @with
+  @subgoal "xs = x' # xs'"
+    @case "x < fst a" @then @have "fst a > fst x'"
+  @endgoal @end   
 @qed
 
 section {* Deleting from a list of pairs *}
@@ -162,55 +161,46 @@ fun remove_elt_pairs :: "'a \<Rightarrow> ('a \<times> 'b) list \<Rightarrow> ('
 | "remove_elt_pairs x (y # ys) = (if fst y = x then ys else y # remove_elt_pairs x ys)"
 setup {* fold add_rewrite_rule @{thms remove_elt_pairs.simps} *}
 
-theorem remove_elt_pairs_map [rewrite]:
+lemma remove_elt_pairs_map [rewrite]:
   "strict_sorted (map fst ys) \<Longrightarrow> map_of_alist (remove_elt_pairs x ys) = delete_map x (map_of_alist ys)"
-@proof
-  @induct ys @with
-    @subgoal "ys = y # ys'"
-      @case "fst y = x" @with @have "x \<notin> set (map fst ys')" @end
-    @endgoal
-  @end
+@proof @induct ys @with
+  @subgoal "ys = y # ys'"
+    @case "fst y = x" @with @have "x \<notin> set (map fst ys')" @end
+  @endgoal @end
 @qed
 
-theorem remove_elt_pairs_on_set [rewrite]:
+lemma remove_elt_pairs_on_set [rewrite]:
   "strict_sorted (map fst ys) \<Longrightarrow> set (map fst (remove_elt_pairs x ys)) = set (map fst ys) - {x}"
 @proof @induct ys @qed
 
-theorem remove_elt_pairs_sorted [backward]:
+lemma remove_elt_pairs_sorted [backward]:
   "strict_sorted (map fst ys) \<Longrightarrow> strict_sorted (map fst (remove_elt_pairs x ys))"
 @proof @induct ys @qed
 
-theorem remove_elt_pairs_idem [rewrite]:
+lemma remove_elt_pairs_idem [rewrite]:
   "x \<notin> set (map fst ys) \<Longrightarrow> remove_elt_pairs x ys = ys"
 @proof @induct ys @qed
 
-theorem remove_elt_pairs_binary [rewrite]:
+lemma remove_elt_pairs_binary [rewrite]:
   "strict_sorted (map fst (xs @ [a] @ ys)) \<Longrightarrow> remove_elt_pairs x (xs @ [a] @ ys) =
     (if x < fst a then (remove_elt_pairs x xs) @ [a] @ ys
      else if x > fst a then xs @ [a] @ remove_elt_pairs x ys else xs @ ys)"
-@proof
-  @induct xs @with
-    @subgoal "xs = []"
-      @case "x < fst a" @with @have "x \<notin> set (map fst ys)" @end
-    @endgoal
-  @end
+@proof @induct xs @with
+  @subgoal "xs = []"
+    @case "x < fst a" @with @have "x \<notin> set (map fst ys)" @end
+  @endgoal @end
 @qed
 
-section {* Merge sort *}
+section {* Search in a list of pairs *}
 
-fun merge_list :: "('a::ord) list \<Rightarrow> 'a list \<Rightarrow> 'a list" where
-  "merge_list xs [] = xs"
-| "merge_list [] ys = ys"
-| "merge_list (x # xs) (y # ys) = (
-    if x \<le> y then x # (merge_list xs (y # ys))
-    else y # (merge_list (x # xs) ys))"
-setup {* fold add_rewrite_rule @{thms merge_list.simps} *}
-setup {* add_fun_induct_rule (@{term_pat "merge_list (?a0.0::?'a::ord list) ?a1.0"}, @{thm merge_list.induct}) *}
-
-theorem merge_list_correct [rewrite]: "set (merge_list xs ys) = set xs \<union> set ys"
-@proof @fun_induct "merge_list xs ys" @qed
-
-theorem merge_list_sorted [backward2]: "sorted xs \<Longrightarrow> sorted ys \<Longrightarrow> sorted (merge_list xs ys)"
-@proof @fun_induct "merge_list xs ys" @qed
+lemma map_of_alist_binary [rewrite]:
+  "strict_sorted (map fst (xs @ [a] @ ys)) \<Longrightarrow> (map_of_alist (xs @ [a] @ ys))\<langle>x\<rangle> =
+   (if x < fst a then (map_of_alist xs)\<langle>x\<rangle>
+    else if x > fst a then (map_of_alist ys)\<langle>x\<rangle> else Some (snd a))"
+@proof @induct xs @with
+  @subgoal "xs = []"
+  @case "x \<notin> set (map fst ys)"
+  @endgoal @end
+@qed
 
 end
